Start transition to Linden group maps for tree interpretation
Groups.v: prepare translation from MatchState to group maps
Semantics.v: replace first_branch' with first_branch and group operations with GroupMap.*
Tree.v: implement direction in interpretation of Linden trees
LWEquivTMatcherDef.v: rephrase equivalence with Linden tree interpretation
TMatching.v: replace call to tree_res' with translating to Linden group map, calling tree_res and converting result back to Warblre capture list

Semantics/Tree.v
@@ -3,7 +3,7 @@ Import ListNotations.
 
 From Linden Require Import Regex Chars Groups.
 From Coq Require Import PeanoNat.
-From Warblre Require Import Typeclasses Parameters.
+From Warblre Require Import Typeclasses Parameters Base.
 
 
 (* A tree represents all the possible paths that could be explored by a backtracking engine *)
@@ -117,82 +117,88 @@ Section Tree.
 
   Definition leaf: Type := (group_map).
 
+  Definition advance_idx (idx: nat) (dir: Direction) :=
+    match dir with
+    | forward => idx+1
+    | backward => idx-1
+    end.
+
   (* returning the highest-priority result *)
   (* we also return the corresponding group map *)
-  Fixpoint tree_res (t:tree) (gm:group_map) (idx:nat): option leaf :=
+  Fixpoint tree_res (t:tree) (gm:group_map) (idx:nat) (dir: Direction): option leaf :=
     match t with
     | Mismatch => None
     | Match => Some gm
     | Choice t1 t2 =>
-        seqop (tree_res t1 gm idx) (tree_res t2 gm idx)
-    | Read c t1 => tree_res t1 gm (idx + 1)
+        seqop (tree_res t1 gm idx dir) (tree_res t2 gm idx dir)
+    | Read c t1 => tree_res t1 gm (advance_idx idx dir) dir
     | CheckFail _ => None
-    | CheckPass _ t1 => tree_res t1 gm idx
-    | GroupAction g t1 => tree_res t1 (GroupMap.update idx g gm) idx
+    | CheckPass _ t1 => tree_res t1 gm idx dir
+    | GroupAction g t1 => tree_res t1 (GroupMap.update idx g gm) idx dir
     | LK lk tlk t1 =>
         match (positivity lk) with
         | true => 
-            match tree_res tlk gm idx with
+            match tree_res tlk gm idx (lk_dir lk) with
             | None => None
             (* using the captures defined in the first branch of the lookahead *)
-            | Some gm' => tree_res t1 gm' idx
+            | Some gm' => tree_res t1 gm' idx dir
             end
         | false =>
-            match tree_res tlk gm idx with
+            match tree_res tlk gm idx (lk_dir lk) with
             (* using previous captures *)
-            | None => tree_res t1 gm idx
+            | None => tree_res t1 gm idx dir
             | Some _ => None
             end
         end
     | LKFail _ _ => None
     | AnchorFail _ => None
-    | AnchorPass _ t => tree_res t gm idx
-    | ReadBackRef _ t => tree_res t gm idx
+    | AnchorPass _ t => tree_res t gm idx dir
+    | ReadBackRef _ t => tree_res t gm idx dir
     end.
 
   (* initializing on a the empty group map *)
   Definition first_branch (t:tree) : option leaf :=
-    tree_res t GroupMap.empty 0.
+    tree_res t GroupMap.empty 0 forward.
 
   (** * All Tree Results *)
 
   (* returns the ordered list of all results of a tree *)
   (* together with the corresponding group map *)
-  Fixpoint tree_leaves (t:tree) (gm:group_map) (idx:nat): list leaf :=
+  Fixpoint tree_leaves (t:tree) (gm:group_map) (idx:nat) (dir: Direction): list leaf :=
     match t with
     | Mismatch => []
     | Match => [gm]
     | Choice t1 t2 =>
-        tree_leaves t1 gm idx ++ tree_leaves t2 gm idx
-    | Read c t1 => tree_leaves t1 gm (idx + 1)
+        tree_leaves t1 gm idx dir ++ tree_leaves t2 gm idx dir
+    | Read c t1 => tree_leaves t1 gm (advance_idx idx dir) dir
     | CheckFail _ => []
-    | CheckPass _ t1 => tree_leaves t1 gm idx
-    | GroupAction g t1 => tree_leaves t1 (GroupMap.update idx g gm) idx
+    | CheckPass _ t1 => tree_leaves t1 gm idx dir
+    | GroupAction g t1 => tree_leaves t1 (GroupMap.update idx g gm) idx dir
     | LK lk tlk t1 =>
         match (positivity lk) with (* Do we want to explore all the branches of the lookahead tree that succeed? *)
         | true =>
-            match (tree_leaves tlk gm idx) with
+            match (tree_leaves tlk gm idx (lk_dir lk)) with
             | [] => []             (* should not happen *)
             (* using the captures defined in the first branch of the lookaround *)
-            | gm'::_ => tree_leaves t1 gm' idx
+            | gm'::_ => tree_leaves t1 gm' idx dir
             end
         | false =>
-            match (tree_leaves tlk gm idx) with
+            match (tree_leaves tlk gm idx (lk_dir lk)) with
             (* using previous captures *)
-            | [] => tree_leaves t1 gm idx
+            | [] => tree_leaves t1 gm idx dir
             | _ => []              (* should not happen *)
             end
         end
     | LKFail _ _ => []
     | AnchorFail _ => []
-    | AnchorPass _ t => tree_leaves t gm idx
-    | ReadBackRef _ t => tree_leaves t gm idx
+    | AnchorPass _ t => tree_leaves t gm idx dir
+    | ReadBackRef _ t => tree_leaves t gm idx dir
     end.
 
 
   (* Property that this definition coincides on the first element with the previous definition given a tree. *)
   Definition first_tree_leaf_prop (t: tree): Prop :=
-    forall gm idx, tree_res t gm idx = hd_error (tree_leaves t gm idx).
+    forall gm idx dir, tree_res t gm idx dir = hd_error (tree_leaves t gm idx dir).
 
 
   (* intermediate lemma about hd_error *)
@@ -214,8 +220,8 @@ Section Tree.
       first_tree_leaf_prop (LK lk tlk t1).
   Proof.
     intros lk tlk t1 Hpos IHtlk IHt1.
-    unfold first_tree_leaf_prop in *. intros gm idx. simpl. rewrite Hpos.
-    specialize (IHtlk gm idx). destruct (tree_res tlk gm idx); destruct (tree_leaves tlk gm idx); try discriminate; simpl in *. 2: reflexivity.
+    unfold first_tree_leaf_prop in *. intros gm idx dir. simpl. rewrite Hpos.
+    specialize (IHtlk gm idx (lk_dir lk)). destruct (tree_res tlk gm idx (lk_dir lk)); destruct (tree_leaves tlk gm idx (lk_dir lk)); try discriminate; simpl in *. 2: reflexivity.
     injection IHtlk as <-; auto.
   Qed.
 
@@ -226,19 +232,19 @@ Section Tree.
       first_tree_leaf_prop (LK lk tlk t1).
   Proof.
     intros lk tlk t1 Hpos IHtlk IHt1.
-    unfold first_tree_leaf_prop in *. intros gm idx. simpl. rewrite Hpos.
-    specialize (IHtlk gm idx). destruct (tree_res tlk gm idx); destruct (tree_leaves tlk gm idx); try discriminate; auto.
+    unfold first_tree_leaf_prop in *. intros gm idx dir. simpl. rewrite Hpos.
+    specialize (IHtlk gm idx (lk_dir lk)). destruct (tree_res tlk gm idx); destruct (tree_leaves tlk gm idx); try discriminate; auto.
   Qed.
 
 
   (* this definition coincides on the first element with the previous definition *)
   Theorem first_tree_leaf:
-    forall t gm idx,
-      tree_res t gm idx = hd_error (tree_leaves t gm idx).
+    forall t gm idx dir,
+      tree_res t gm idx dir = hd_error (tree_leaves t gm idx dir).
   Proof.
     intros t. induction t; intros. 1-7,9-11: simpl; auto.
     - rewrite IHt1. rewrite IHt2. rewrite hd_error_app. unfold seqop.
-      destruct (hd_error (tree_leaves t1 gm idx)) eqn:HD; auto.
+      destruct (hd_error (tree_leaves t1 gm idx dir)) eqn:HD; auto.
     - destruct (positivity lk) eqn:Hlkpos. + now apply first_tree_leaf_poslk. + now apply first_tree_leaf_neglk.
     - simpl. auto.
   Qed.
@@ -252,8 +258,8 @@ Section Tree.
 
   (* Group map irrelevance property for a given tree. *)
   Definition leaves_group_map_indep_prop (t: tree): Prop :=
-    forall gm1 gm2 idx1 idx2,
-      tree_leaves t gm1 idx1 = [] -> tree_leaves t gm2 idx2 = [].
+    forall gm1 gm2 idx1 idx2 dir1 dir2,
+      tree_leaves t gm1 idx1 dir1 = [] -> tree_leaves t gm2 idx2 dir2 = [].
 
   (* Intermediate lemma for positive lookarounds *)
   Lemma leaves_group_map_indep_poslk:
@@ -262,10 +268,10 @@ Section Tree.
       leaves_group_map_indep_prop (LK lk tlk t1).
   Proof.
     intros lk tlk t1 Hposlk IHtlk IHt1; unfold leaves_group_map_indep_prop in *; simpl.
-    rewrite Hposlk. intros gm1 gm2 idx1 idx2 Hnil1.
-    specialize (IHtlk gm1 gm2 idx1 idx2). destruct (tree_leaves tlk gm1 idx1) as [|gm' q]; simpl in *.
+    rewrite Hposlk. intros gm1 gm2 idx1 idx2 dir1 dir2 Hnil1.
+    specialize (IHtlk gm1 gm2 idx1 idx2 (lk_dir lk) (lk_dir lk)). destruct (tree_leaves tlk gm1 idx1 _) as [|gm' q]; simpl in *.
     1: { specialize (IHtlk eq_refl). now rewrite IHtlk. }
-    destruct (tree_leaves tlk gm2 idx2) as [|gm'0 q0]; simpl in *. 1: reflexivity.
+    destruct (tree_leaves tlk gm2 idx2 _) as [|gm'0 q0]; simpl in *. 1: reflexivity.
     eapply IHt1; eauto.
   Qed.
 
@@ -276,24 +282,24 @@ Section Tree.
       leaves_group_map_indep_prop (LK lk tlk t1).
   Proof.
     intros lk tlk t1 Hposlk IHtlk IHt1; unfold leaves_group_map_indep_prop in *; simpl.
-    rewrite Hposlk. intros gm1 gm2 idx1 idx2 Hnil1.
-    destruct (tree_leaves tlk gm1 idx1) as [|gm' q] eqn:Hnilsub1; simpl in *.
-    1: { specialize (IHtlk gm1 gm2 idx1 idx2 Hnilsub1). rewrite IHtlk. eapply IHt1; eauto. }
-    destruct (tree_leaves tlk gm2 idx2) as [|gm'0 q0] eqn:Hnilsub2; simpl in *. 2: reflexivity.
-    exfalso. apply IHtlk with (gm2 := gm1) (idx2 := idx1) in Hnilsub2. congruence.
+    rewrite Hposlk. intros gm1 gm2 idx1 idx2 dir1 dir2 Hnil1.
+    destruct (tree_leaves tlk gm1 idx1 _) as [|gm' q] eqn:Hnilsub1; simpl in *.
+    1: { specialize (IHtlk gm1 gm2 idx1 idx2 (lk_dir lk) (lk_dir lk) Hnilsub1). rewrite IHtlk. eapply IHt1; eauto. }
+    destruct (tree_leaves tlk gm2 idx2 _) as [|gm'0 q0] eqn:Hnilsub2; simpl in *. 2: reflexivity.
+    exfalso. apply IHtlk with (gm2 := gm1) (idx2 := idx1) (dir2 := lk_dir lk) in Hnilsub2. congruence.
   Qed.
 
 
   Lemma leaves_group_map_indep:
-    forall t gm1 gm2 idx1 idx2,
-      tree_leaves t gm1 idx1 = [] -> tree_leaves t gm2 idx2 = [].
+    forall t gm1 gm2 idx1 idx2 dir1 dir2,
+      tree_leaves t gm1 idx1 dir1 = [] -> tree_leaves t gm2 idx2 dir2 = [].
   Proof.
     intros t.
     induction t; intros. 1-7,9-11: simpl; auto;
       simpl in H; try solve[inversion H];
       try solve[eapply IHt in H; eauto].
     - apply app_eq_nil in H as [NIL1 NIL2].
-      apply IHt1 with (gm2:=gm2) (idx2:=idx2) in NIL1. apply IHt2 with (gm2:=gm2) (idx2:=idx2) in NIL2.
+      apply IHt1 with (gm2:=gm2) (idx2:=idx2) (dir2 := dir2) in NIL1. apply IHt2 with (gm2:=gm2) (idx2:=idx2) (dir2 := dir2) in NIL2.
       rewrite NIL1. rewrite NIL2. auto.
     - destruct (positivity lk) eqn:Hlkpos. + eapply leaves_group_map_indep_poslk; eauto. + eapply leaves_group_map_indep_neglk; eauto.
     - eapply IHt in H. eauto.
